Little bit more work on local variables

utp/utp_lvar.thy
@@ -30,7 +30,24 @@ definition lvar_lift :: "('a \<Longrightarrow> 'b) \<Rightarrow> ('a, '\<alpha>)
 "lvar_lift X = \<lparr> lens_get = \<lambda> s. \<lparr> lvar\<^sub>u = get\<^bsub>X\<^esub> (lvar\<^sub>u s), \<dots> = more s \<rparr>
                , lens_put = \<lambda> s v. \<lparr> lvar\<^sub>u = put\<^bsub>X\<^esub> (lvar\<^sub>u s) (lvar\<^sub>u v), \<dots> = more v \<rparr> \<rparr>"
 
+term "lvar_lift x \<times>\<^sub>L lvar_lift x"
+
+term "lvar_lift snd\<^sub>L"
+
+term "(lvar_lift snd\<^sub>L \<times>\<^sub>L lvar_lift snd\<^sub>L)"
+
+term "P \<restriction>\<^sub>p (lvar_lift snd\<^sub>L \<times>\<^sub>L lvar_lift snd\<^sub>L)"
+
+abbreviation lvlift :: "_ \<Rightarrow> _" ("\<lceil>_\<rceil>\<^sub>l") where "\<lceil>P\<rceil>\<^sub>l \<equiv> P \<oplus>\<^sub>p (lvar_lift snd\<^sub>L \<times>\<^sub>L lvar_lift snd\<^sub>L)"
+abbreviation lvdrop :: "_ \<Rightarrow> _" ("\<lfloor>_\<rfloor>\<^sub>l") where "\<lfloor>P\<rfloor>\<^sub>l \<equiv> P \<restriction>\<^sub>p (lvar_lift snd\<^sub>L \<times>\<^sub>L lvar_lift snd\<^sub>L)"
+
+text {* Lens representing local variables *}
+
 definition "lvar = VAR lvar\<^sub>u"
+
+text {* Lens representing global variables *}
+
+definition "gvar = VAR more"
 
 declare lvar_def [upred_defs]
 
@@ -40,15 +57,37 @@ lemma uvar_lvar [simp]: "uvar lvar"
 lemma vwb_lens_uvar_lift [simp]: "vwb_lens X \<Longrightarrow> vwb_lens (lvar_lift X)"
   by (unfold_locales, simp_all add: lvar_lift_def)
 
+lemma uvar_gvar [simp]: "uvar gvar"
+  by (simp add: gvar_def, unfold_locales, simp_all)
+
+lemma lvar_indep_gvar [simp]: "lvar \<bowtie> gvar" "gvar \<bowtie> lvar"
+  by (auto intro:lens_indepI simp add: lvar_def gvar_def)
+
 definition var_scope :: 
   "(('a \<Longrightarrow> ('a \<times> '\<L>, '\<alpha>) lvar_scheme) \<Rightarrow> (('a \<times> '\<L>, '\<alpha>) lvar_scheme) hrelation) \<Rightarrow>
    (('\<L>, '\<alpha>) lvar_scheme) hrelation" where
 "var_scope P = (\<^bold>+(lvar_lift snd\<^sub>L) ;; P (fst\<^sub>L ;\<^sub>L lvar) ;; \<^bold>-(lvar_lift snd\<^sub>L))"
 
 syntax
-  "_var_scope" :: "id \<Rightarrow> type \<Rightarrow> logic \<Rightarrow> logic" ("var _ : _ \<bullet> _" [0,0,100] 100)
+  "_var_scope" :: "id \<Rightarrow> logic \<Rightarrow> logic" ("var _ \<bullet> _" [0,10] 10)
+  "_var_scope_ty" :: "id \<Rightarrow> type \<Rightarrow> logic \<Rightarrow> logic" ("var _ : _ \<bullet> _" [0,0,10] 10)
 
 translations
-  "var x : 'a \<bullet> P" == "CONST var_scope (\<lambda> x :: ('a \<Longrightarrow> _). P)"
+  "var x \<bullet> P" == "CONST var_scope (\<lambda> x. P)"
+  "var x : 'a \<bullet> P" => "CONST var_scope (\<lambda> x :: ('a \<Longrightarrow> _). P)"
+
+lemma lvar_assign_null:
+  "(var x \<bullet> x := v) = II"
+  apply (simp add: var_scope_def lvar_lift_def upred_defs urel_defs relcomp_unfold lens_comp_def fst_lens_def snd_lens_def)
+  apply (transfer, simp add: relcomp_unfold, rule ext, simp add:prod.case_eq_if)
+  apply (metis (no_types, lifting) fst_conv lvar.equality lvar.ext_inject lvar.select_convs(1) lvar.update_convs(1) sndI)
+done
+
+lemma "\<lbrakk> $lvar \<sharp> Q; $lvar\<acute> \<sharp> Q \<rbrakk> \<Longrightarrow> (var x \<bullet> P x ;; Q) = ((var x \<bullet> P x) ;; \<lfloor>Q\<rfloor>\<^sub>l)"
+  apply (simp add: var_scope_def lvar_lift_def upred_defs urel_defs relcomp_unfold lens_comp_def fst_lens_def snd_lens_def prod_lens_def prod.case_eq_if)
+  apply (transfer, simp add: relcomp_unfold prod.case_eq_if lens_create_def comp_def, rule ext)
+  apply (safe)
+  apply (simp)
+  oops
 
 end
